refactor: simplify `dfoldrM`

Batteries/Data/Fin/Basic.lean
@@ -18,47 +18,21 @@ alias enum := Array.finRange
 @[deprecated (since := "2024-11-15")]
 alias list := List.finRange
 
-/-- Dependent version of `Fin.foldlM`. -/
-@[inline] def dfoldlM [Monad m] (n : Nat) (α : Fin (n + 1) → Sort _)
-    (f : ∀ (i : Fin n), α i.castSucc → m (α i.succ)) (init : α 0) : m (α (last n)) :=
-  loop 0 (Nat.zero_lt_succ n) init where
-  /-- Inner loop for `Fin.dfoldlM`.
-    ```
-  Fin.foldM.loop n α f i h xᵢ = do
-    let xᵢ₊₁ ← f i xᵢ
-    ...
-    let xₙ ← f (n-1) xₙ₋₁
-    pure xₙ
-  ```
-  -/
-  @[semireducible] loop (i : Nat) (h : i < n + 1) (x : α ⟨i, h⟩) : m (α (last n)) :=
-    if h' : i < n then
-      (f ⟨i, h'⟩ x) >>= loop (i + 1) (Nat.succ_lt_succ h')
-    else
-      haveI : ⟨i, h⟩ = last n := by ext; simp; omega
-      _root_.cast (congrArg (fun i => m (α i)) this) (pure x)
+/-- Dependent version of `Fin.foldr`. -/
+@[inline] def dfoldr (n : Nat) (α : Fin (n + 1) → Sort _)
+    (f : ∀ (i : Fin n), α i.succ → α i.castSucc) (init : α (last n)) : α 0 :=
+  loop n (Nat.lt_succ_self n) init where
+  /-- Inner loop for `Fin.dfoldr`.
+    `Fin.dfoldr.loop n α f i h x = f 0 (f 1 (... (f i x)))`  -/
+  @[specialize] loop (i : Nat) (h : i < n + 1) (x : α ⟨i, h⟩) : α 0 :=
+    match i with
+    | i + 1 => loop i (Nat.lt_of_succ_lt h) (f ⟨i, Nat.lt_of_succ_lt_succ h⟩ x)
+    | 0 => x
 
 /-- Dependent version of `Fin.foldrM`. -/
 @[inline] def dfoldrM [Monad m] (n : Nat) (α : Fin (n + 1) → Sort _)
     (f : ∀ (i : Fin n), α i.succ → m (α i.castSucc)) (init : α (last n)) : m (α 0) :=
-  loop n (Nat.lt_succ_self n) init where
-  /-- Inner loop for `Fin.foldRevM`.
-    ```
-  Fin.foldRevM.loop n α f i h xᵢ = do
-    let xᵢ₋₁ ← f (i+1) xᵢ
-    ...
-    let x₁ ← f 1 x₂
-    let x₀ ← f 0 x₁
-    pure x₀
-  ```
-  -/
-  @[semireducible] loop (i : Nat) (h : i < n + 1) (x : α ⟨i, h⟩) : m (α 0) :=
-    if h' : i > 0 then
-      (f ⟨i - 1, by omega⟩ (by simpa [Nat.sub_one_add_one_eq_of_pos h'] using x))
-        >>= loop (i - 1) (by omega)
-    else
-      haveI : ⟨i, h⟩ = 0 := by ext; simp; omega
-      _root_.cast (congrArg (fun i => m (α i)) this) (pure x)
+  dfoldr n (fun i => m (α i)) (fun i x => x >>= f i) (pure init)
 
 /-- Dependent version of `Fin.foldl`. -/
 @[inline] def dfoldl (n : Nat) (α : Fin (n + 1) → Sort _)
@@ -72,13 +46,22 @@ alias list := List.finRange
       haveI : ⟨i, h⟩ = last n := by ext; simp; omega
       _root_.cast (congrArg α this) x
 
-/-- Dependent version of `Fin.foldr`. -/
-@[inline] def dfoldr (n : Nat) (α : Fin (n + 1) → Sort _)
-    (f : ∀ (i : Fin n), α i.succ → α i.castSucc) (init : α (last n)) : α 0 :=
-  loop n (Nat.lt_succ_self n) init where
-  /-- Inner loop for `Fin.dfoldr`.
-    `Fin.dfoldr.loop n α f i h x = f 0 (f 1 (... (f i x)))`  -/
-  @[specialize] loop (i : Nat) (h : i < n + 1) (x : α ⟨i, h⟩) : α 0 :=
-    match i with
-    | i + 1 => loop i (Nat.lt_of_succ_lt h) (f ⟨i, Nat.lt_of_succ_lt_succ h⟩ x)
-    | 0 => x
+/-- Dependent version of `Fin.foldlM`. -/
+@[inline] def dfoldlM [Monad m] (n : Nat) (α : Fin (n + 1) → Sort _)
+    (f : ∀ (i : Fin n), α i.castSucc → m (α i.succ)) (init : α 0) : m (α (last n)) :=
+  loop 0 (Nat.zero_lt_succ n) init where
+  /-- Inner loop for `Fin.dfoldlM`.
+    ```
+  Fin.foldM.loop n α f i h xᵢ = do
+    let xᵢ₊₁ ← f i xᵢ
+    ...
+    let xₙ ← f (n-1) xₙ₋₁
+    pure xₙ
+  ```
+  -/
+  @[semireducible, specialize] loop (i : Nat) (h : i < n + 1) (x : α ⟨i, h⟩) : m (α (last n)) :=
+    if h' : i < n then
+      (f ⟨i, h'⟩ x) >>= loop (i + 1) (Nat.succ_lt_succ h')
+    else
+      haveI : ⟨i, h⟩ = last n := by ext; simp; omega
+      _root_.cast (congrArg (fun i => m (α i)) this) (pure x)
