Batteries/Data/Fin/Fold.lean
@@ -8,74 +8,49 @@ import Batteries.Data.Fin.Basic
 
 namespace Fin
 
-/-! ### dfoldlM -/
+/-! ### dfoldr -/
 
-theorem dfoldlM_loop_lt [Monad m] (f : ∀ (i : Fin n), α i.castSucc → m (α i.succ)) (h : i < n) (x) :
-    dfoldlM.loop n α f i (Nat.lt_add_right 1 h) x =
-      (f ⟨i, h⟩ x) >>= (dfoldlM.loop n α f (i+1) (Nat.add_lt_add_right h 1)) := by
-  rw [dfoldlM.loop, dif_pos h]
+theorem dfoldr_loop_zero (f : (i : Fin n) → α i.succ → α i.castSucc) (x) :
+    dfoldr.loop n α f 0 (Nat.zero_lt_succ n) x = x := rfl
 
-theorem dfoldlM_loop_eq [Monad m] (f : ∀ (i : Fin n), α i.castSucc → m (α i.succ)) (x) :
-    dfoldlM.loop n α f n (Nat.le_refl _) x = pure x := by
-  rw [dfoldlM.loop, dif_neg (Nat.lt_irrefl _), cast_eq]
+theorem dfoldr_loop_succ (f : (i : Fin n) → α i.succ → α i.castSucc) (h : i < n) (x) :
+      dfoldr.loop n α f (i+1) (Nat.add_lt_add_right h 1) x =
+        dfoldr.loop n α f i (Nat.lt_add_right 1 h) (f ⟨i, h⟩ x) := rfl
 
-@[simp] theorem dfoldlM_zero [Monad m] (f : (i : Fin 0) → α i.castSucc → m (α i.succ)) (x) :
-    dfoldlM 0 α f x = pure x := dfoldlM_loop_eq ..
+theorem dfoldr_loop (f : (i : Fin (n+1)) → α i.succ → α i.castSucc) (h : i+1 ≤ n+1) (x) :
+      dfoldr.loop (n+1) α f (i+1) (Nat.add_lt_add_right h 1) x =
+        f 0 (dfoldr.loop n (α ∘ succ) (f ·.succ) i h x) := by
+  induction i with
+  | zero => rfl
+  | succ i ih => exact ih ..
 
-theorem dfoldlM_loop [Monad m] (f : (i : Fin (n+1)) → α i.castSucc → m (α i.succ)) (h : i < n+1)
-    (x) : dfoldlM.loop (n+1) α f i (Nat.lt_add_right 1 h) x =
-      f ⟨i, h⟩ x >>= (dfoldlM.loop n (α ∘ succ) (f ·.succ ·) i h .) := by
-  if h' : i < n then
-    rw [dfoldlM_loop_lt _ h _]
-    congr; funext
-    rw [dfoldlM_loop_lt _ h' _, dfoldlM_loop]; rfl
-  else
-    cases Nat.le_antisymm (Nat.le_of_lt_succ h) (Nat.not_lt.1 h')
-    rw [dfoldlM_loop_lt]
-    congr; funext
-    rw [dfoldlM_loop_eq, dfoldlM_loop_eq]
+@[simp] theorem dfoldr_zero (f : (i : Fin 0) → α i.succ → α i.castSucc) (x) :
+    dfoldr 0 α f x = x := rfl
 
-theorem dfoldlM_succ [Monad m] (f : (i : Fin (n+1)) → α i.castSucc → m (α i.succ)) (x) :
-    dfoldlM (n+1) α f x = f 0 x >>= (dfoldlM n (α ∘ succ) (f ·.succ ·) .) :=
-  dfoldlM_loop ..
+theorem dfoldr_succ (f : (i : Fin (n+1)) → α i.succ → α i.castSucc) (x) :
+    dfoldr (n+1) α f x = f 0 (dfoldr n (α ∘ succ) (f ·.succ) x) := dfoldr_loop ..
 
-theorem dfoldlM_eq_foldlM [Monad m] (f : (i : Fin n) → α → m α) (x : α) :
-    dfoldlM n (fun _ => α) f x = foldlM n (fun x i => f i x) x := by
-  induction n generalizing x with
-  | zero => simp only [dfoldlM_zero, foldlM_zero]
-  | succ n ih =>
-    simp only [dfoldlM_succ, foldlM_succ, Function.comp_apply, Function.comp_def]
-    congr; ext; simp only [ih]
+theorem dfoldr_succ_last (f : (i : Fin (n+1)) → α i.succ → α i.castSucc) (x) :
+    dfoldr (n+1) α f x = dfoldr n (α ∘ castSucc) (f ·.castSucc) (f (last n) x) := by
+  induction n with
+  | zero => simp only [dfoldr_succ, dfoldr_zero, last, zero_eta]
+  | succ n ih => rw [dfoldr_succ, ih (α := α ∘ succ) (f ·.succ), dfoldr_succ]; congr
+
+theorem dfoldr_eq_dfoldrM (f : (i : Fin n) → α i.succ → α i.castSucc) (x) :
+    dfoldr n α f x = dfoldrM (m:=Id) n α f x := rfl
+
+theorem dfoldr_eq_foldr (f : Fin n → α → α) (x : α) : dfoldr n (fun _ => α) f x = foldr n f x := by
+  induction n with
+  | zero => simp only [dfoldr_zero, foldr_zero]
+  | succ n ih => simp only [dfoldr_succ, foldr_succ, Function.comp_apply, Function.comp_def, ih]
 
 /-! ### dfoldrM -/
 
-theorem dfoldrM_loop_zero [Monad m] (f : (i : Fin n) → α i.succ → m (α i.castSucc)) (x) :
-    dfoldrM.loop n α f 0 (Nat.zero_lt_succ n) x = pure x := by
-  rw [dfoldrM.loop, dif_neg (Nat.not_lt_zero _), cast_eq]
-
-theorem dfoldrM_loop_succ [Monad m] (f : (i : Fin n) → α i.succ → m (α i.castSucc)) (h : i < n)
-    (x) : dfoldrM.loop n α f (i+1) (Nat.add_lt_add_right h 1) x =
-      f ⟨i, h⟩ x >>= dfoldrM.loop n α f i (Nat.lt_add_right 1 h) := by
-  rw [dfoldrM.loop, dif_pos (Nat.zero_lt_succ i)]
-  simp only [Nat.add_one_sub_one, castSucc_mk, succ_mk, eq_mpr_eq_cast, cast_eq]
-
-theorem dfoldrM_loop [Monad m] [LawfulMonad m] (f : (i : Fin (n+1)) → α i.succ → m (α i.castSucc))
-    (h : i+1 ≤ n+1) (x) : dfoldrM.loop (n+1) α f (i+1) (Nat.add_lt_add_right h 1) x =
-      dfoldrM.loop n (α ∘ succ) (f ·.succ) i h x >>= f 0 := by
-  induction i with
-  | zero =>
-    rw [dfoldrM_loop_zero, dfoldrM_loop_succ, pure_bind]
-    conv => rhs; rw [←bind_pure (f 0 x)]
-    congr
-  | succ i ih =>
-    rw [dfoldrM_loop_succ _ h, dfoldrM_loop_succ _ (Nat.succ_lt_succ_iff.mp h), bind_assoc]
-    congr; funext; exact ih ..
-
 @[simp] theorem dfoldrM_zero [Monad m] (f : (i : Fin 0) → α i.succ → m (α i.castSucc)) (x) :
-    dfoldrM 0 α f x = pure x := dfoldrM_loop_zero ..
+    dfoldrM 0 α f x = pure x := rfl
 
-theorem dfoldrM_succ [Monad m] [LawfulMonad m] (f : (i : Fin (n+1)) → α i.succ → m (α i.castSucc))
-    (x) : dfoldrM (n+1) α f x = dfoldrM n (α ∘ succ) (f ·.succ) x >>= f 0 := dfoldrM_loop ..
+theorem dfoldrM_succ [Monad m] (f : (i : Fin (n+1)) → α i.succ → m (α i.castSucc))
+    (x) : dfoldrM (n+1) α f x = dfoldrM n (α ∘ succ) (f ·.succ) x >>= f 0 := dfoldr_succ ..
 
 theorem dfoldrM_eq_foldrM [Monad m] [LawfulMonad m] (f : (i : Fin n) → α → m α) (x : α) :
     dfoldrM n (fun _ => α) f x = foldrM n f x := by
@@ -126,47 +101,44 @@ theorem dfoldl_eq_foldl (f : Fin n → α → α) (x : α) :
     simp only [dfoldl_succ, foldl_succ, Function.comp_apply, Function.comp_def]
     congr; simp only [ih]
 
-/-! ### dfoldr -/
+/-! ### dfoldlM -/
 
-theorem dfoldr_loop_zero (f : (i : Fin n) → α i.succ → α i.castSucc) (x) :
-    dfoldr.loop n α f 0 (Nat.zero_lt_succ n) x = x := by
-  rw [dfoldr.loop]
+theorem dfoldlM_loop_lt [Monad m] (f : ∀ (i : Fin n), α i.castSucc → m (α i.succ)) (h : i < n) (x) :
+    dfoldlM.loop n α f i (Nat.lt_add_right 1 h) x =
+      (f ⟨i, h⟩ x) >>= (dfoldlM.loop n α f (i+1) (Nat.add_lt_add_right h 1)) := by
+  rw [dfoldlM.loop, dif_pos h]
 
-theorem dfoldr_loop_succ (f : (i : Fin n) → α i.succ → α i.castSucc) (h : i < n) (x) :
-      dfoldr.loop n α f (i+1) (Nat.add_lt_add_right h 1) x =
-        dfoldr.loop n α f i (Nat.lt_add_right 1 h) (f ⟨i, h⟩ x) := by
-  rw [dfoldr.loop]
+theorem dfoldlM_loop_eq [Monad m] (f : ∀ (i : Fin n), α i.castSucc → m (α i.succ)) (x) :
+    dfoldlM.loop n α f n (Nat.le_refl _) x = pure x := by
+  rw [dfoldlM.loop, dif_neg (Nat.lt_irrefl _), cast_eq]
 
-theorem dfoldr_loop (f : (i : Fin (n+1)) → α i.succ → α i.castSucc) (h : i+1 ≤ n+1) (x) :
-      dfoldr.loop (n+1) α f (i+1) (Nat.add_lt_add_right h 1) x =
-        f 0 (dfoldr.loop n (α ∘ succ) (f ·.succ) i h x) := by
-  induction i with
-  | zero => simp [dfoldr_loop_succ, dfoldr_loop_zero]
-  | succ i ih => rw [dfoldr_loop_succ _ h, dfoldr_loop_succ _ (Nat.succ_lt_succ_iff.mp h),
-      ih (Nat.le_of_succ_le h)]; rfl
+@[simp] theorem dfoldlM_zero [Monad m] (f : (i : Fin 0) → α i.castSucc → m (α i.succ)) (x) :
+    dfoldlM 0 α f x = pure x := dfoldlM_loop_eq ..
 
-@[simp] theorem dfoldr_zero (f : (i : Fin 0) → α i.succ → α i.castSucc) (x) :
-    dfoldr 0 α f x = x := dfoldr_loop_zero ..
+theorem dfoldlM_loop [Monad m] (f : (i : Fin (n+1)) → α i.castSucc → m (α i.succ)) (h : i < n+1)
+    (x) : dfoldlM.loop (n+1) α f i (Nat.lt_add_right 1 h) x =
+      f ⟨i, h⟩ x >>= (dfoldlM.loop n (α ∘ succ) (f ·.succ ·) i h .) := by
+  if h' : i < n then
+    rw [dfoldlM_loop_lt _ h _]
+    congr; funext
+    rw [dfoldlM_loop_lt _ h' _, dfoldlM_loop]; rfl
+  else
+    cases Nat.le_antisymm (Nat.le_of_lt_succ h) (Nat.not_lt.1 h')
+    rw [dfoldlM_loop_lt]
+    congr; funext
+    rw [dfoldlM_loop_eq, dfoldlM_loop_eq]
 
-theorem dfoldr_succ (f : (i : Fin (n+1)) → α i.succ → α i.castSucc) (x) :
-    dfoldr (n+1) α f x = f 0 (dfoldr n (α ∘ succ) (f ·.succ) x) := dfoldr_loop ..
+theorem dfoldlM_succ [Monad m] (f : (i : Fin (n+1)) → α i.castSucc → m (α i.succ)) (x) :
+    dfoldlM (n+1) α f x = f 0 x >>= (dfoldlM n (α ∘ succ) (f ·.succ ·) .) :=
+  dfoldlM_loop ..
 
-theorem dfoldr_succ_last (f : (i : Fin (n+1)) → α i.succ → α i.castSucc) (x) :
-    dfoldr (n+1) α f x = dfoldr n (α ∘ castSucc) (f ·.castSucc) (f (last n) x) := by
-  induction n with
-  | zero => simp only [dfoldr_succ, dfoldr_zero, last, zero_eta]
-  | succ n ih => rw [dfoldr_succ, ih (α := α ∘ succ) (f ·.succ), dfoldr_succ]; congr
-
-theorem dfoldr_eq_dfoldrM (f : (i : Fin n) → α i.succ → α i.castSucc) (x) :
-    dfoldr n α f x = dfoldrM (m:=Id) n α f x := by
-  induction n <;> simp [dfoldr_succ, dfoldrM_succ, *]
-
-theorem dfoldr_eq_foldr (f : Fin n → α → α) (x : α) : dfoldr n (fun _ => α) f x = foldr n f x := by
-  induction n with
-  | zero => simp only [dfoldr_zero, foldr_zero]
-  | succ n ih => simp only [dfoldr_succ, foldr_succ, Function.comp_apply, Function.comp_def, ih]
-
--- TODO: add `dfoldl_rev` and `dfoldr_rev`
+theorem dfoldlM_eq_foldlM [Monad m] (f : (i : Fin n) → α → m α) (x : α) :
+    dfoldlM n (fun _ => α) f x = foldlM n (fun x i => f i x) x := by
+  induction n generalizing x with
+  | zero => simp only [dfoldlM_zero, foldlM_zero]
+  | succ n ih =>
+    simp only [dfoldlM_succ, foldlM_succ, Function.comp_apply, Function.comp_def]
+    congr; ext; simp only [ih]
 
 /-! ### `Fin.fold{l/r}{M}` equals `List.fold{l/r}{M}` -/
 
